Split the definitions in Inc.v in different files for sharing Imp defs between Hoare and Inc

theories/Inc.v
@@ -11,236 +11,10 @@ Require Import Ltac2.Option.
 
 Require Import StringAsOT.
 Require Import StateMap.
+Require Import Imp.
+Require Import Hoare.
 
 Import ListNotations.
- 
-Inductive aexp : Type :=
-  | ANum (n : nat)
-  | AId (x : string)
-  | APlus (a1 a2 : aexp)
-.
-
-Inductive bexp : Type :=
-  | BTrue
-  | BFalse
-  | BEq (a1 a2 : aexp)
-  | BNot (b : bexp)
-.
-
-Inductive com : Type :=
-  | Skip
-  | Asign: string -> aexp -> com
-  | Seq : com -> com -> com
-  | Assume : bexp -> com
-  | Error: com
-  | Star: com -> com
-  | Choice: com -> com -> com.
-
-Coercion AId : string >-> aexp.
-
-Coercion ANum : nat >-> aexp.
-
-Declare Custom Entry com.
-Declare Scope com_scope.
-Notation "<{ e }>" := e (at level 0, e custom com at level 99) : com_scope.
-Notation "( x )" := x (in custom com, x at level 99) : com_scope.
-Notation "x" := x (in custom com at level 0, x constr at level 0) : com_scope.
-Notation "f x .. y" := (.. (f x) .. y)
-                  (in custom com at level 0, only parsing,
-                  f constr at level 0, x constr at level 9,
-                  y constr at level 9) : com_scope.
-Notation "x + y" := (APlus x y) (in custom com at level 50, left associativity).
-Notation "'true'" := true (at level 1).
-Notation "'true'" := BTrue (in custom com at level 0).
-Notation "'false'" := false (at level 1).
-Notation "'false'" := BFalse (in custom com at level 0).
-Notation "x = y" := (BEq x y) (in custom com at level 70, no associativity).
-Notation "'~' b" := (BNot b) (in custom com at level 75, right associativity).
-Open Scope com_scope.
-
-(* Eval compute in  InA_cons_hd M.E ("Y"%string :: "X"%string :: nil). *)
-
-(* witch to aevalR *)
-Fixpoint aeval (st : state) (a : aexp) : option nat :=
-  match a with
-  | ANum n => Some n
-  | AId x => StateMap.get st x
-  | <{a1 + a2}> => 
-      match (aeval st a1), (aeval st a2) with
-      | Some va1, Some va2 => Some (va1 + va2)
-      | _, _ => None
-      end
-  end.
-
-Definition equal_option [A B] (eq : A -> B -> bool) (a : option A) (b : option B) : bool
-  := match a with
-     | None => match b with
-               | None => true
-               | _ => false
-               end
-     | Some a => match b with
-                 | Some b => eq a b
-                 | _ => false
-                 end
-     end.
-
-Fixpoint beval (st : state) (b : bexp): bool :=
-  match b with
-  | BTrue => true
-  | BFalse => false
-  | BEq a1 a2 => equal_option (Nat.eqb) (aeval st a1) (aeval st a2)
-  | BNot b1 => negb (beval st b1)
-  end.
-
-
-Reserved  Notation "'assume' l " 
-          (in custom com at level 8, l custom com at level 0).
-Reserved Notation "x ; y" (in custom com at level 90, right associativity).
-
-Notation "x := y" :=
-         (Asign x y)
-            (in custom com at level 0, x constr at level 0,
-             y at level 85, no associativity) : com_scope.
-Notation "'local' x " :=
-        (Asign x (ANum 0))
-          (in custom com at level 8, x custom com at level 0) : com_scope.
-Notation "'skip'" :=
-         Skip (in custom com at level 0) : com_scope.
-Notation "x ; y" :=
-         (Seq x y)
-          (in custom com at level 90, right associativity) : com_scope.
-Notation "'assume' l " :=
-        (Assume l)
-          (in custom com at level 8, l custom com at level 0) : com_scope.
-Notation "'error()'" :=
-          Error (in custom com at level 0) : com_scope.
-Notation "c '⋆'" :=
-        (Star c) (in custom com at level 8) : com_scope.
-Notation "x '⨁' y " :=
-        (Choice x y) (in custom com at level 8) : com_scope.
-
-(* Notations for while, if and assert keywords *)
-
-Definition While b c := <{ (assume b ; c)⋆ ; assume ~ b }>.
-
-Notation "'while' b 'do' c" :=
-  (While b c)
-  (in custom com at level 10, b at next level, c at next level) : com_scope.
-
-Definition If b c c' := <{ (assume b ; c) ⨁ ((assume ~ b) ; c') }>.
-
-Notation "'if' b 'then' c 'else' c'" :=
-  (If b c c')
-  (in custom com at level 10, c at next level, c' at next level) : com_scope.
-
-Definition Assert b := <{ (assume b) ⨁ ((assume ~ b) ; error()) }>.
-
-Notation "'assert' '(' c ')' " :=
-  (Assert c) (in custom com at level 8) : com_scope.
-
-Definition Assertion := state -> Prop.
-
-Definition Aexp : Type := state -> option nat.
-Definition assert_of_Prop (P : Prop) : Assertion := fun _ => P.
-Definition Aexp_of_nat (n : nat) : Aexp := fun _ => Some n.
-Definition Aexp_of_aexp (a : aexp) : Aexp := fun st => aeval st a.
-
-(* Sortclass, the class of sorts; its objects are the terms whose type is a sort (e.g. Prop or Type).  *)
-Coercion assert_of_Prop : Sortclass >-> Assertion.
-Coercion Aexp_of_nat : nat >-> Aexp.
-Coercion Aexp_of_aexp : aexp >-> Aexp.
-
-Arguments assert_of_Prop /.
-Arguments Aexp_of_nat /.
-Arguments Aexp_of_aexp /.
-Add Printing Coercion Aexp_of_nat Aexp_of_aexp assert_of_Prop.
-
-Declare Scope assertion_scope.
-Bind Scope assertion_scope with Assertion.
-Bind Scope assertion_scope with Aexp.
-Delimit Scope assertion_scope with assertion.
-Notation assertion P := (P%assertion : Assertion).
-Notation mkAexp a := (a%assertion : Aexp).
-Notation "~ P" := (fun st => ~ assertion P st) : assertion_scope.
-Notation "P /\ Q" := (fun st => assertion P st /\  assertion Q st) : assertion_scope.
-Notation "P \/ Q" := (fun st => assertion P st \/ assertion Q st) : assertion_scope.
-Notation "P -> Q" := (fun st => assertion P st -> assertion Q st) : assertion_scope.
-Notation "P <-> Q" := (fun st => assertion P st <-> assertion Q st) : assertion_scope.
-Notation "a = b" := (fun st => mkAexp a st = mkAexp b st) : assertion_scope.
-Notation "a + b" := (fun st => mkAexp a st + mkAexp b st) : assertion_scope.
-
-
-Definition assert_implies (P Q : Assertion) : Prop :=
-  forall st, P st -> Q st.
-
-Declare Scope inclogic_spec_scope.
-
-Notation "P ->> Q" := (assert_implies P Q)
-                      (at level 80) : inclogic_spec_scope.
-Open Scope inclogic_spec_scope.
-
-Notation "P <<->> Q" :=
-  (P ->> Q /\ Q ->> P) (at level 80) : inclogic_spec_scope. 
-
-
-(* Notation "'if' B 'then' T else E" :=
-  ((assume (B) ; C) ⨁ (assume (~B) ; C))
-  in custom com at level 80) : com_scope. *)
-
-(* Notation "'assert' B" :=
-  (assume (B) ⨁ (assume (~B) ; error()))
-  in custom com at level 80) : com_scope. *)
-
-
-Reserved Notation
-         "st '=[' c ']=>' ϵ ':' st'"
-         (at level 40, c custom com at level 99,
-          st constr, ϵ constr at next level).
-
-
-Inductive Signal: Type := 
-| ok
-| err.
-
-Inductive ceval : com -> state -> Signal -> state -> Prop :=
-| E_Skip : forall st,
-  st =[ skip ]=> ok : st
-| E_Local : forall st x y,
-  st =[ local x ]=> ok : (x !-> y ; st)
-| E_Asgn : forall st a n x,
-  aeval st a = Some n ->
-  st =[ x := a ]=> ok : (x !-> n ; st)
-(* Alternative version
-| E_Asgn : forall st a n x st',
-  aeval st a = n ->
-  st' = (x !-> n ; st) ->
-  st =[ x := a ]=> ok : st' *)
-| E_Seq_Norm : forall c1 c2 st st' st'' ϵ,
-  st =[ c1 ]=> ok : st' ->
-  st' =[ c2 ]=> ϵ : st'' ->
-  st =[ c1 ; c2 ]=> ϵ : st''
-| E_Seq_Err : forall c1 c2 st st',
-  st =[ c1 ]=> err : st' ->
-  st =[ c1 ; c2 ]=> err : st'
- | E_Assume : forall st b,
-  beval st b = true ->
-  st =[ assume b ]=> ok : st
-| E_Error: forall st,
-  st =[ error() ]=> err: st
-| E_StarZero : forall c st ϵ,
-  st =[ c ⋆ ]=> ϵ : st
-| E_StarNonZero : forall c st st' ϵ,
-  st =[ c ⋆ ; c  ]=> ϵ : st' ->
-  st =[ c ⋆ ]=> ϵ : st'
-| E_ChoiceLeft: forall x y st st' ϵ,
-  st =[ x ]=> ϵ : st' ->
-  st =[ x ⨁ y ]=> ϵ : st'
-| E_ChoiceRight: forall x y st st' ϵ,
-  st =[ y ]=> ϵ : st' ->
-  st =[ x ⨁ y ]=> ϵ : st'
-where "st =[ c ]=> ϵ : st'" := (ceval c st ϵ st').
-
-Local Hint Constructors ceval : core.
 
 Definition Inc_triple
            (P : Assertion) (c : com) (s: Signal) (Q: Assertion): Prop :=
@@ -255,6 +29,8 @@ Notation "[[ P ]] c [[ ϵ ↑ Q ]]" :=
 Notation "[[ P ]] c [[ ok ↑ Q ]] [[ err ↑ R ]] " :=
   ([[ P ]] c [[ ok ↑ Q ]] /\ [[ P ]] c [[ err ↑ R ]]) (at level 90, c custom com at level 99): inclogic_spec_scope.
 
+
+Local Hint Constructors ceval : core.
 
 (*
   [p]C1[ok:q] [q]C2[ϵ:r]
@@ -544,7 +320,7 @@ Theorem DeriveIteration : forall P c ε Q b,
   forall x, x < b -> [[ P ]] Cpow x c [[ ε ↑ Q ]] ->
   [[ P ]] c ⋆ [[ ε ↑ fun st' => x < b -> Q st' ]].
 Proof with auto.
-  intros P c ε Q b x H HCstarSeq st HQ.
+  (* intros P c ε Q b x H HCstarSeq st HQ.
   destruct x.
   - simpl in *. exists st.
     specialize (HQ H).
@@ -560,7 +336,7 @@ Proof with auto.
     apply lt_succ_l in H.
     exists st'.
 
-    admit.
+    admit. *)
     (* apply IHx H  *)
   (* specialize (HCstarSeq st' HQ) as [ st [ Heval HP ] ]. *)
   (* inversion Heval; subst; eauto.   *)
@@ -687,6 +463,7 @@ match y with
   | Error => Error
   | Star c => Star (aux c)
   | Choice c1 c2 => Choice (aux c1) (aux c2)
+  | CLocal x' c' => if_y_eq x' (CLocal yvar (aux c')) (CLocal x' (aux c'))
   end
 | w => 
   match c with
@@ -697,6 +474,7 @@ match y with
   | Error => Error
   | Star c => Star (aux c)
   | Choice c1 c2 => Choice (aux c1) (aux c2)
+  | CLocal x' c' => (CLocal x' (aux c'))
   end
 end.
 
@@ -711,6 +489,20 @@ Example testsubstCmd2: substCmd "X"%string (APlus (ANum 1) (ANum 1))
   = <{ "Y" := (APlus (ANum 1) (ANum 1)); skip; "Z" := (APlus (ANum 1) (APlus (ANum 1) (ANum 1)))}>.
 Proof. reflexivity. Qed.
 
+
+
+(* Local Variable
+
+  [p] C (y/x) [ϵ:q]
+  ------------------------- y ∈ Free(p, C)  
+  [p] local x. C [ε: ∃y. q]
+*)
+Theorem LocalVariable : forall P Q F (C: com) (y: aexp) (x: string) ε,
+  [[ P ]] substCmd x y C [[ ε ↑ Q ]]
+  ->
+  [[ P /\ F ]] local x . C [[ ε ↑ Q /\ F ]].
+Proof.
+Admitted.
 
 (* x is free in p if p is invariant under changing x
   : i.e., σ ∈ p ⇔ ∀ v. (σ | x ↦ v) ∈ p, where (σ | x ↦ v) for the 
@@ -761,14 +553,19 @@ split.
 assumption.
 Admitted.
 
-
 Theorem Subst1 : forall P Q c ε e x,
   [[ P ]] c [[ ε ↑ Q ]]
   ->
-  [[ P [e |-> x] ]] c [[ ε ↑ Q [e |-> x ] ]].
+  [[ P [x |-> e] ]] substCmd x e c [[ ε ↑ Q [x |-> e ] ]].
 Proof.
 Admitted.
 
+Theorem Subst2 : forall P Q c ε y x,
+  [[ P ]] c [[ ε ↑ Q ]]
+  ->
+  [[ P [x |-> y] ]] substCmd x y c [[ ε ↑ Q [x |-> y ] ]].
+Proof.
+Admitted.
 
 (*  Local BEGIN VAR V1; · · · VAR Vn; C END
   Semantics: command C is executed, then the values of V1, · · · , Vn
@@ -803,17 +600,6 @@ Admitted.
 Declare Scope hoare_spec_scope.
 
 Open Scope hoare_spec_scope.
-
-Definition hoare_triple
-           (P : Assertion) (c : com) (s: Signal) (Q : Assertion) : Prop :=
-  forall st st',
-     st =[ c ]=> s: st' ->
-     P st ->
-     Q st'.
-
-Notation "{{ P }} c {{ ε Q }}" :=
-(hoare_triple P c ε Q) (at level 90, c custom com at level 99)
-  : hoare_spec_scope.
 
 (* Principle of Agreement : [u]c[u'] ∧ u ⇒ o ∧ {o}c{o'} ⇒ u' => o' *)
 Lemma Agreement: forall IPRe IPost c ε HPre HPost, [[IPRe]] c [[ ε ↑ IPost ]] /\ IPRe ->> HPre /\ (hoare_triple HPre c ε HPost) -> IPost ->> HPost.
