theories/Hoare.v
@@ -1,0 +1,13 @@
+Require Import StringAsOT.
+Require Import StateMap.
+Require Import Imp.
+
+Definition hoare_triple
+           (P : Assertion) (c : com) (s: Signal) (Q : Assertion) : Prop :=
+  forall st st',
+     st =[ c ]=> s: st' ->
+     P st ->
+     Q st'.
+
+Notation "{{ P }} c {{ ε ↑ Q }}" :=
+(hoare_triple P c ε Q) (at level 90, c custom com at level 99): inclogic_spec_scope.
