theories/Imp.v
@@ -1,0 +1,227 @@
+Require Export Coq.Strings.String.
+Require Import StateMap.
+
+Inductive aexp : Type :=
+  | ANum (n : nat)
+  | AId (x : string)
+  | APlus (a1 a2 : aexp)
+.
+
+Inductive bexp : Type :=
+  | BTrue
+  | BFalse
+  | BEq (a1 a2 : aexp)
+  | BNot (b : bexp)
+.
+
+Inductive com : Type :=
+  | Skip
+  | Asign: string -> aexp -> com
+  | Seq : com -> com -> com
+  | Assume : bexp -> com
+  | Error: com
+  | Star: com -> com
+  | Choice: com -> com -> com
+  | CLocal: string -> com -> com.
+
+Coercion AId : string >-> aexp.
+
+Coercion ANum : nat >-> aexp.
+
+Declare Custom Entry com.
+Declare Scope com_scope.
+Notation "<{ e }>" := e (at level 0, e custom com at level 99) : com_scope.
+Notation "( x )" := x (in custom com, x at level 99) : com_scope.
+Notation "x" := x (in custom com at level 0, x constr at level 0) : com_scope.
+Notation "f x .. y" := (.. (f x) .. y)
+                  (in custom com at level 0, only parsing,
+                  f constr at level 0, x constr at level 9,
+                  y constr at level 9) : com_scope.
+Notation "x + y" := (APlus x y) (in custom com at level 50, left associativity).
+Notation "'true'" := true (at level 1).
+Notation "'true'" := BTrue (in custom com at level 0).
+Notation "'false'" := false (at level 1).
+Notation "'false'" := BFalse (in custom com at level 0).
+Notation "x = y" := (BEq x y) (in custom com at level 70, no associativity).
+Notation "'~' b" := (BNot b) (in custom com at level 75, right associativity).
+Open Scope com_scope.
+
+(* Eval compute in  InA_cons_hd M.E ("Y"%string :: "X"%string :: nil). *)
+
+(* witch to aevalR *)
+Fixpoint aeval (st : state) (a : aexp) : option nat :=
+  match a with
+  | ANum n => Some n
+  | AId x => StateMap.get st x
+  | <{a1 + a2}> => 
+      match (aeval st a1), (aeval st a2) with
+      | Some va1, Some va2 => Some (va1 + va2)
+      | _, _ => None
+      end
+  end.
+
+Definition equal_option [A B] (eq : A -> B -> bool) (a : option A) (b : option B) : bool
+  := match a with
+     | None => match b with
+               | None => true
+               | _ => false
+               end
+     | Some a => match b with
+                 | Some b => eq a b
+                 | _ => false
+                 end
+     end.
+
+Fixpoint beval (st : state) (b : bexp): bool :=
+  match b with
+  | BTrue => true
+  | BFalse => false
+  | BEq a1 a2 => equal_option (Nat.eqb) (aeval st a1) (aeval st a2)
+  | BNot b1 => negb (beval st b1)
+  end.
+
+Reserved  Notation "'assume' l " 
+          (in custom com at level 8, l custom com at level 0).
+Reserved Notation "x ; y" (in custom com at level 90, right associativity).
+
+Notation "x := y" :=
+         (Asign x y)
+            (in custom com at level 0, x constr at level 0,
+             y at level 85, no associativity) : com_scope.
+Notation "'local' x . C" :=
+        (CLocal x C)
+          (in custom com at level 8, x custom com at level 0) : com_scope.
+Notation "'skip'" :=
+         Skip (in custom com at level 0) : com_scope.
+Notation "x ; y" :=
+         (Seq x y)
+          (in custom com at level 90, right associativity) : com_scope.
+Notation "'assume' l " :=
+        (Assume l)
+          (in custom com at level 8, l custom com at level 0) : com_scope.
+Notation "'error()'" :=
+          Error (in custom com at level 0) : com_scope.
+Notation "c '⋆'" :=
+        (Star c) (in custom com at level 8) : com_scope.
+Notation "x '⨁' y " :=
+        (Choice x y) (in custom com at level 8) : com_scope.
+
+(* Notations for while, if and assert keywords *)
+
+Definition While b c := <{ (assume b ; c)⋆ ; assume ~ b }>.
+
+Notation "'while' b 'do' c" :=
+  (While b c)
+  (in custom com at level 10, b at next level, c at next level) : com_scope.
+
+Definition If b c c' := <{ (assume b ; c) ⨁ ((assume ~ b) ; c') }>.
+
+Notation "'if' b 'then' c 'else' c'" :=
+  (If b c c')
+  (in custom com at level 10, c at next level, c' at next level) : com_scope.
+
+Definition Assert b := <{ (assume b) ⨁ ((assume ~ b) ; error()) }>.
+
+Notation "'assert' '(' c ')' " :=
+  (Assert c) (in custom com at level 8) : com_scope.
+
+
+Reserved Notation
+         "st '=[' c ']=>' ϵ ':' st'"
+         (at level 40, c custom com at level 99,
+          st constr, ϵ constr at next level).
+
+
+Inductive Signal: Type := 
+| ok
+| err.
+
+Inductive ceval : com -> state -> Signal -> state -> Prop :=
+| E_Skip : forall st,
+  st =[ skip ]=> ok : st
+| E_SkipF :
+  empty =[ skip ]=> err : empty
+| E_Local : forall st st' x v c ϵ,
+  (x !-> v ; st) =[ local x . c ]=> ϵ : (x !-> v ; st')
+| E_Asgn : forall st a n x,
+  aeval st a = Some n ->
+  st =[ x := a ]=> ok : (x !-> n ; st)
+(* Alternative version
+| E_Asgn : forall st a n x st',
+  aeval st a = n ->
+  st' = (x !-> n ; st) ->
+  st =[ x := a ]=> ok : st' *)
+| E_Seq_Norm : forall c1 c2 st st' st'' ϵ,
+  st =[ c1 ]=> ok : st' ->
+  st' =[ c2 ]=> ϵ : st'' ->
+  st =[ c1 ; c2 ]=> ϵ : st''
+| E_Seq_Err : forall c1 c2 st st',
+  st =[ c1 ]=> err : st' ->
+  st =[ c1 ; c2 ]=> err : st'
+ | E_Assume : forall st b,
+  beval st b = true ->
+  st =[ assume b ]=> ok : st
+| E_ErrorOk:
+  empty =[ error() ]=> ok: empty
+| E_Error: forall st,
+  st =[ error() ]=> err: st
+| E_StarZero : forall c st ϵ,
+  st =[ c ⋆ ]=> ϵ : st
+| E_StarNonZero : forall c st st' ϵ,
+  st =[ c ⋆ ; c  ]=> ϵ : st' ->
+  st =[ c ⋆ ]=> ϵ : st'
+| E_ChoiceLeft: forall x y st st' ϵ,
+  st =[ x ]=> ϵ : st' ->
+  st =[ x ⨁ y ]=> ϵ : st'
+| E_ChoiceRight: forall x y st st' ϵ,
+  st =[ y ]=> ϵ : st' ->
+  st =[ x ⨁ y ]=> ϵ : st'
+where "st =[ c ]=> ϵ : st'" := (ceval c st ϵ st').
+
+Local Hint Constructors ceval : core.
+
+
+Definition Assertion := state -> Prop.
+
+Definition Aexp : Type := state -> option nat.
+Definition assert_of_Prop (P : Prop) : Assertion := fun _ => P.
+Definition Aexp_of_nat (n : nat) : Aexp := fun _ => Some n.
+Definition Aexp_of_aexp (a : aexp) : Aexp := fun st => aeval st a.
+
+(* Sortclass, the class of sorts; its objects are the terms whose type is a sort (e.g. Prop or Type).  *)
+Coercion assert_of_Prop : Sortclass >-> Assertion.
+Coercion Aexp_of_nat : nat >-> Aexp.
+Coercion Aexp_of_aexp : aexp >-> Aexp.
+
+Arguments assert_of_Prop /.
+Arguments Aexp_of_nat /.
+Arguments Aexp_of_aexp /.
+Add Printing Coercion Aexp_of_nat Aexp_of_aexp assert_of_Prop.
+
+Declare Scope assertion_scope.
+Bind Scope assertion_scope with Assertion.
+Bind Scope assertion_scope with Aexp.
+Delimit Scope assertion_scope with assertion.
+Notation assertion P := (P%assertion : Assertion).
+Notation mkAexp a := (a%assertion : Aexp).
+Notation "~ P" := (fun st => ~ assertion P st) : assertion_scope.
+Notation "P /\ Q" := (fun st => assertion P st /\  assertion Q st) : assertion_scope.
+Notation "P \/ Q" := (fun st => assertion P st \/ assertion Q st) : assertion_scope.
+Notation "P -> Q" := (fun st => assertion P st -> assertion Q st) : assertion_scope.
+Notation "P <-> Q" := (fun st => assertion P st <-> assertion Q st) : assertion_scope.
+Notation "a = b" := (fun st => mkAexp a st = mkAexp b st) : assertion_scope.
+Notation "a + b" := (fun st => mkAexp a st + mkAexp b st) : assertion_scope.
+
+
+Definition assert_implies (P Q : Assertion) : Prop :=
+  forall st, P st -> Q st.
+
+Declare Scope inclogic_spec_scope.
+
+Notation "P ->> Q" := (assert_implies P Q)
+                      (at level 80) : inclogic_spec_scope.
+Open Scope inclogic_spec_scope.
+
+Notation "P <<->> Q" :=
+  (P ->> Q /\ Q ->> P) (at level 80) : inclogic_spec_scope. 
+
